ok

SStructTT/SStruct/SrtOrder.lean
@@ -19,6 +19,59 @@ instance {S : Type} {s : S} [ord : SrtOrder S] : Decidable (s ∈ ord.weaken_set
 instance {S : Type} {s : S} [ord : SrtOrder S] : Decidable (s ∈ ord.contra_set) :=
   ord.contra_dec s
 
+section CoverSet
+variable {Srt : Type} [ord : SrtOrder Srt]
+
+def CoverSet (s : Srt) : Set Srt :=
+  fun s' =>
+    (s ∈ ord.weaken_set -> s' ∈ ord.weaken_set) ∧
+    (s ∈ ord.contra_set -> s' ∈ ord.contra_set)
+
+lemma CoverSet.self_mem {s : Srt} : s ∈ CoverSet s := by
+  constructor <;> simp
+
+lemma CoverSet.min_mem {s : Srt} : ord.e ∈ CoverSet s := by
+  constructor
+  . intro; apply ord.e_weaken
+  . intro; apply ord.e_contra
+
+lemma CoverSet.weaken {s1 s2 : Srt} :
+    s1 ∈ CoverSet s2 -> s2 ∈ ord.weaken_set -> s1 ∈ ord.weaken_set := by
+  intro h1 h2; cases h1; aesop
+
+lemma CoverSet.contra {s1 s2 : Srt} :
+    s1 ∈ CoverSet s2 -> s2 ∈ ord.contra_set -> s1 ∈ ord.contra_set := by
+  intro h1 h2; cases h1; aesop
+
+lemma CoverSet.lower_mem {s1 s2 : Srt} :
+    s1 <= s2 -> s1 ∈ CoverSet s2 := by
+  intro le
+  constructor
+  case left  => intro h; apply ord.weaken_set.lower le h
+  case right => intro h; apply ord.contra_set.lower le h
+
+lemma CoverSet.lower_subset {s1 s2 : Srt} :
+    s1 <= s2 -> CoverSet s1 ⊆ CoverSet s2 := by
+  intro le s c1
+  constructor
+  case left =>
+    intro h; have ⟨h1, h2⟩ := c1
+    have := ord.weaken_set.lower le h
+    aesop
+  case right =>
+    intro h; have ⟨h1, h2⟩ := c1
+    have := ord.contra_set.lower le h
+    aesop
+
+lemma CoverSet.trans {s1 s2 s3 : Srt} :
+    s2 ∈ CoverSet s1 -> s3 ∈ CoverSet s2 -> s3 ∈ CoverSet s1 := by
+  intro h1 h2
+  constructor
+  case left  => intro h; cases h1; cases h2; aesop
+  case right => intro h; cases h1; cases h2; aesop
+
+end CoverSet
+
 namespace SO4 -- 4 Sorted
 inductive Srt where
   | U -- unbound
@@ -189,4 +242,5 @@ instance : SrtOrder Srt where
   e_contra := Srt.contra.U
   weaken_dec := Srt.weaken_dec
   contra_dec := Srt.contra_dec
+
 end SO4
